new approach to external connection proofs
We can prove juicy-dry entirely at the logic level.

veric/SequentialClight.v
@@ -94,11 +94,70 @@ Proof.
       iApply (step_fupdN_mono with "IH"); eauto.
 Qed.
 
+Definition ext_spec_entails {M E Z} (es1 es2 : external_specification M E Z) :=
+  (forall e x1 p tys args z m, ext_spec_pre es1 e x1 p tys args z m ->
+     exists x2, ext_spec_pre es2 e x2 p tys args z m /\
+       forall ty ret z' m', ext_spec_post es2 e x2 p ty ret z' m' ->
+                            ext_spec_post es1 e x1 p ty ret z' m') /\
+  (forall v z m, ext_spec_exit es1 v z m -> ext_spec_exit es2 v z m).
+
+Theorem ext_spec_entails_safe : forall {G C M Z} {genv_symb} Hcore es1 es2 ge n z c m
+  (Hes : ext_spec_entails es1 es2),
+  @step_lemmas.dry_safeN G C M Z genv_symb Hcore es1 ge n z c m -> @step_lemmas.dry_safeN G C M Z genv_symb Hcore es2 ge n z c m.
+Proof.
+  induction n as [n IHn] using lt_wf_ind; intros.
+  inv H.
+  - constructor.
+  - eapply step_lemmas.safeN_step; eauto.
+    eapply IHn; eauto.
+  - destruct Hes as (Hes & ?).
+    apply Hes in H1 as (x2 & ? & ?).
+    eapply step_lemmas.safeN_external; eauto; intros.
+    edestruct H2 as (c' & ? & ?); eauto.
+    exists c'; split; auto.
+    eapply IHn; eauto; [lia | by split].
+  - destruct Hes.
+    eapply step_lemmas.safeN_halted; eauto.
+Qed.
+
+Definition sig_of_funspec {Σ} (f : @funspec Σ) := typesig2signature (typesig_of_funspec f) (callingconvention_of_funspec f).
+
+Lemma juicy_dry_spec : forall `{!VSTGS OK_ty Σ} ext_link fs es
+  (Hspecs : forall s f, In (ext_link s, f) fs -> match f with mk_funspec ts cc E A P Q =>
+     let e := EF_external s (typesig2signature ts cc) in
+     forall w p tys args m z, exists x,
+       state_interp m z ∗ P w (filter_genv (symb2genv p), args) ⊢ ⌜ext_spec_pre es e x p tys args z m⌝ ∧
+         ∀ ty ret z' m', ⌜ext_spec_post es e x p ty ret z' m'⌝ → |==>
+           state_interp m' z' ∗ Q w (make_ext_rval (filter_genv (symb2genv p)) ty ret)
+   end)
+  (Hexit : forall v z m, ext_spec_exit es v z m),
+  ext_spec_entails (add_funspecs_rec OK_ty ext_link (void_spec OK_ty) fs) es.
+Proof.
+  intros; constructor; last done; clear Hexit.
+  intros *; intros Hpre; induction fs; simpl; first done.
+  destruct a as (i, [[]]); simpl in *.
+  rewrite /funspec2pre in Hpre; rewrite /funspec2post; if_tac.
+  - clear IHfs.
+    destruct e; inv H.
+    specialize (Hspecs _ _ ltac:(eauto)).
+    destruct x1 as ((n, phi), w).
+    specialize (Hspecs w); edestruct Hspecs as (x & Hspec).
+    exists x.
+    destruct Hpre as (Hvalid & Hty & HP).
+    eapply Hspec in HP; last done.
+    revert HP; ouPred.unseal; intros (Hpre & Hpost).
+    split; first apply Hpre.
+    intros ???? Hpost'; eapply Hpost; auto.
+  - apply IHfs; auto.
+    intros; apply Hspecs; auto.
+Qed.
+
 Lemma whole_program_sequential_safety_ext:
-   forall Σ {CS: compspecs} `{!VSTGpreS OK_ty Σ} {OK_spec : ext_spec OK_ty} (initial_oracle: OK_ty)
-     (EXIT: semax_prog.postcondition_allows_exit OK_spec tint)
-     prog V G m,
-     (forall {HH : VSTGS OK_ty Σ}, semax_prog prog initial_oracle V G) ->
+   forall Σ {CS: compspecs} `{!VSTGpreS OK_ty Σ} {Espec : forall `{VSTGS OK_ty Σ}, ext_spec OK_ty} {dryspec : ext_spec OK_ty} (initial_oracle: OK_ty)
+     (EXIT: forall `{!VSTGS OK_ty Σ}, semax_prog.postcondition_allows_exit Espec tint)
+     (Hdry : forall `{!VSTGS OK_ty Σ}, ext_spec_entails Espec dryspec)
+     prog V (G : forall `{VSTGS OK_ty Σ}, funspecs) m,
+     (forall {HH : VSTGS OK_ty Σ}, semax_prog(OK_spec := Espec) prog initial_oracle V G) ->
      Genv.init_mem prog = Some m ->
      exists b, exists q,
        Genv.find_symbol (Genv.globalenv prog) (prog_main prog) = Some b /\
@@ -107,7 +166,7 @@ Lemma whole_program_sequential_safety_ext:
        forall n,
         @dry_safeN _ _ _ OK_ty (genv_symb_injective)
             (cl_core_sem (globalenv prog))
-            OK_spec
+            dryspec
             (Build_genv (Genv.globalenv prog) (prog_comp_env prog))
              n initial_oracle q m.
 Proof.
@@ -118,7 +177,7 @@ Proof.
            0 m q m (Vptr b Ptrofs.zero) nil /\
         @dry_safeN _ _ _ OK_ty (genv_symb_injective)
             (cl_core_sem (globalenv prog))
-            OK_spec
+            dryspec
             (Build_genv (Genv.globalenv prog) (prog_comp_env prog))
              n initial_oracle q m).
   2: { destruct (H1 O) as (b0 & q0 & ? & (? & _) & _); eexists _, _; split; first done; split; first done.
@@ -130,14 +189,15 @@ Proof.
   simpl; intros; iIntros "_".
   iMod (@init_VST _ _ VSTGpreS0) as "H".
   iDestruct ("H" $! Hinv) as (?? HE) "(H & ?)".
-  specialize (H (Build_VSTGS _ _ (HeapGS _ _ _ _) HE)).
-  eapply (semax_prog_rule _ _ _ _ n) in H as (b & q & (? & ? & Hinit & ->) & Hsafe); [| done..].
+  set (HH := Build_VSTGS _ _ (HeapGS _ _ _ _) HE).
+  specialize (H HH); specialize (EXIT HH).
+  eapply (semax_prog_rule _ _ _ _ n) in H as (b & q & (? & ? & Hinit & ->) & Hsafe); [|done..].
   iMod (Hsafe with "H") as "Hsafe".
   rewrite bi.and_elim_l.
   iPoseProof (adequacy with "Hsafe") as "Hsafe".
   iApply step_fupd_intro; first done; iNext.
   iApply (step_fupdN_mono with "Hsafe"); apply bi.pure_mono; intros.
-  eauto 6.
+  eapply ext_spec_entails_safe in H; eauto 6.
 Qed.
 
 Definition fun_id (ext_link: Strings.String.string -> ident) (ef: external_function) : option ident :=
